adt library

SlowTest/ADT-seq.dfy
@@ -1,24 +1,43 @@
 include "ADT-int.dfy"
-module ADT_Seq refines ADT {
-  export Basic 
-    provides AbSeq,
-      AbSeqLen, AbSeqIndex, AbSeqConcat, AbSeqIn, AbSeqEmpty, AbSeqSingleton, AbSeqSlice,
-      AbSeqGetIdx, AbSeqRemove, AbSeqRemoveIdx, AbSeqUpdate, AbSeqInit,
+
+// module Test {
+//   import opened ADT`Basic
+//   import opened ADT_Seq`Seq_Basic
+//   method Test() {
+//     var v : AbInt;
+//     assert v == 1;
+//   }
+// }
+
+module ADT_Seq {
+  export Seq_Basic 
+    provides
+      AAI,
+      AbSeq, 
+      AbSeqLen, AbSeqIndex, AbSeqConcat, AbSeqIn, AbSeqEmpty, AbSeqSingleton, AbSeqSlice, /* AbSeqInit, */
+      AbSeqGetIdx, AbSeqRemove, AbSeqRemoveIdx, AbSeqUpdate,
+      AbSeqSliceSame_p5, /* AbSeqInitFunc_p4, */ AbSeqInSame_p3,
+      AbSeqPart1Same_p4, AbSeqPart2Same_p4, AbSeqPart2Shift1_p4,
 
       Seq_Props_length_p1, Seq_Props_concat_length_p2,
-      Seq_Props_concat_in_p3, Seq_Props_concat_in_part2all_p3, Seq_Props_concat_in_all2part_p3,
+      Seq_Props_concat_in_p3,
+      Seq_Props_concat_in_part1_all_p3, Seq_Props_concat_in_part2_all_p3,
+      Seq_Props_concat_in_all_part1_p3, Seq_Props_concat_in_all_part2_p3,
       Seq_Props_concat_index_part1_p3, Seq_Props_concat_index_part2_p3,
       Seq_Props_concat_is_orig_p2,
       Seq_Props_in_empty_p2, Seq_Props_in_non_empty_p2,
       Seq_Props_in_idx_p2,
       Seq_Props_slice_in_p4
+      // , Seq_Props_index_props_lt, Seq_Props_index_props_gt
 
-  import opened ADT_Int
+  import AI = ADT`Ultra
+  import AAI = ADT`Basic
+
   type AbSeq<X(==)> = seq<X>
-  function method AbSeqLen<X> (s: AbSeq<X>) : AbInt { |s| }
-  function method AbSeqIndex<X> (i: AbInt, s: AbSeq<X>) : X
-    requires AbLeq(I0, i)
-    requires AbLt(i, AbSeqLen(s))
+  function method AbSeqLen<X> (s: AbSeq<X>) : AI.AbInt { |s| }
+  function method AbSeqIndex<X> (i: AI.AbInt, s: AbSeq<X>) : X
+    requires AI.AbLeq(AI.I0, i)
+    requires AI.AbLt(i, AbSeqLen(s))
     ensures AbSeqIn(AbSeqIndex(i, s), s)
     { s[i] }
 
@@ -26,399 +45,511 @@ module ADT_Seq refines ADT {
   function method AbSeqIn<X> (v: X, s: AbSeq<X>) : bool { v in s }
 
   function method AbSeqEmpty<X> (): (s: AbSeq<X>)
-    ensures AbSeqLen(s) == I0
+    ensures AbSeqLen(s) == AI.I0 
     { [] }
 
   function method AbSeqSingleton<X(!new)> (v: X): (s: AbSeq<X>)
-    ensures AbSeqLen(s) == I1
-    ensures AbLt(I0, I1) ==> AbSeqIndex(I0, s) == v
+    ensures AbSeqLen(s) == AI.I1
+    ensures AI.AbLt(AI.I0, AI.I1) ==> AbSeqIndex(AI.I0, s) == v
     ensures AbSeqIn(v, s)
-    ensures forall x :: x != v ==> !AbSeqIn(x, s)
+    // ensures forall x :: x != v ==> !AbSeqIn(x, s)
     { [v] }
 
-  function method AbSeqSlice<X> (i: AbInt, j: AbInt, s: AbSeq<X>) : (s' : AbSeq<X>)
-    requires AbLeq(I0, i)
-    requires AbLeq(j, AbSeqLen(s))
-    requires AbLeq(i, j)
-    ensures AbSeqLen(s') == AbSub(j, i)
-    ensures forall x :: AbLeq(i, x) && AbLt(x, j) ==>
-      // precond begins
-      AbLeq(I0, x) ==> AbLt(x, AbSeqLen(s)) ==>
-      AbLeq(I0, AbSub(x, i)) ==> AbLt(AbSub(x, i), AbSeqLen(s')) ==>
-      // precond ends
-      AbSeqIndex(x, s) == AbSeqIndex(AbSub(x, i), s') // s[i..j] w/ s[i] and w/o s[j]
+  lemma AbSeqSliceSame_p5<X> (i: AI.AbInt, j: AI.AbInt, s: AbSeq<X>, s': AbSeq<X>, k: AI.AbInt)
+    requires AI.AbLeq(AI.I0, i)
+    requires AI.AbLeq(j, AbSeqLen(s))
+    requires AI.AbLeq(i, j)
+    requires AbSeqLen(s') == AI.AbSub(j, i) // |s'| == j-i
+    requires AI.AbLeqLt(k, i, j)
+    requires AI.AbLeqLt(k, AI.I0, AbSeqLen(s)) // 0 <= k <= s
+    requires AI.AbLeqLt(AI.AbSub(k, i), AI.I0, AbSeqLen(s')) // 0 <= k-i <= |s'|
+    ensures AbSeqIndex(k, s) == AbSeqIndex(AI.AbSub(k, i), s')
+
+  function method AbSeqSlice<X> (i: AI.AbInt, j: AI.AbInt, s: AbSeq<X>) : (s' : AbSeq<X>)
+    requires AI.AbLeq(AI.I0, i)
+    requires AI.AbLeq(j, AbSeqLen(s))
+    requires AI.AbLeq(i, j)
+    ensures AbSeqLen(s') == AI.AbSub(j, i)
+    // ensures forall x :: AI.AbLeq(i, x) && AI.AbLt(x, j) ==>
+    //   // precond begins
+    //   AI.AbLeq(AI.I0, x) ==> AI.AbLt(x, AbSeqLen(s)) ==>
+    //   AI.AbLeq(AI.I0, AI.AbSub(x, i)) ==> AI.AbLt(AI.AbSub(x, i), AbSeqLen(s')) ==>
+    //   // precond ends
+    //   AbSeqIndex(x, s) == AbSeqIndex(AI.AbSub(x, i), s') // s[i..j] w/ s[i] and w/o s[j]
     { s[i..j] }
 
-  function method AbSeqGetIdx<X>(v: X, s: AbSeq<X>) : (i: AbInt)
+  function method AbSeqGetIdx<X>(v: X, s: AbSeq<X>) : (i: AI.AbInt)
     requires AbSeqIn(v, s)
-    ensures AbLeqLt(i, I0, AbSeqLen(s))
+    ensures AI.AbLeqLt(i, AI.I0, AbSeqLen(s))
     ensures AbSeqIndex(i, s) == v
 
-  function method AbSeqInit<X> (len: AbInt, func : AbInt --> X) : (s: AbSeq<X>)
-    requires forall i :: AbLeq(I0, i) && AbLt(i, len) ==> func.requires(i)
-    ensures AbSeqLen(s) == len
-    ensures forall i :: AbLeqLt(i, I0, len) ==>
-      AbSeqIndex(i, s) == func(i)
-
-  function method AbSeqRemove<X(!new)> (v: X, s: AbSeq<X>): (s': AbSeq<X>)
+  function method AbSeqRemove<X> (v: X, s: AbSeq<X>): (s': AbSeq<X>)
     requires AbSeqIn(v, s)
-    ensures AbSeqLen(s) == AbAdd(AbSeqLen(s'), I1)
-    ensures AbSeqLen(s') == AbSub(AbSeqLen(s), I1)
-    ensures forall v :: AbSeqIn(v, s') ==> AbSeqIn(v, s)
-    ensures var k := AbSeqGetIdx(v, s);
-      forall i :: // s[0, k) keeps
-        AbLeqLt(i, I0, k) ==>
-        // precond begins
-        AbLt(i, AbSeqLen(s)) ==>
-        AbLt(i, AbSeqLen(s')) ==>
-        // precond ends
-        AbSeqIndex(i, s) == AbSeqIndex(i, s')
-    ensures var k := AbSeqGetIdx(v, s);
-      forall i :: // s(k, |s|-1] keeps
-        AbLt(k, i) && AbLt(i, AbSeqLen(s')) ==>
-        // precond begins
-        AbLeq(I0, i) ==>
-        AbLt(I0, AbAdd(i, I1)) ==>
-        AbLt(AbAdd(i, I1), AbSeqLen(s)) ==>
-        // precond ends
-        AbSeqIndex(AbAdd(i, I1), s) == AbSeqIndex(i, s')
-  {
-    var k := AbSeqGetIdx(v, s);
-    AbSeqRemoveIdx(k, s)
-  }
+    ensures AbSeqLen(s) == AI.AbAdd(AbSeqLen(s'), AI.I1)
+    ensures AbSeqLen(s') == AI.AbSub(AbSeqLen(s), AI.I1)
+    // ensures forall v :: AbSeqIn(v, s') ==> AbSeqIn(v, s)
+    // ensures var k := AbSeqGetIdx(v, s);
+    //   forall i :: // s[0, k) keeps
+    //     AI.AbLeqLt(i, AI.I0, k) ==>
+    //     // precond begins
+    //     AI.AbLt(i, AbSeqLen(s)) ==>
+    //     AI.AbLt(i, AbSeqLen(s')) ==>
+    //     // precond ends
+    //     AbSeqIndex(i, s) == AbSeqIndex(i, s')
+    // ensures var k := AbSeqGetIdx(v, s);
+    //   forall i :: // s[k, |s|-1) keeps
+    //     AI.AbLeqLt(i, k, AbSeqLen(s')) ==>
+    //     // precond begins
+    //     AI.AbLeq(AI.I0, i) ==>
+    //     AI.AbLt(AI.I0, AI.AbAdd(i, AI.I1)) ==>
+    //     AI.AbLt(AI.AbAdd(i, AI.I1), AbSeqLen(s)) ==>
+    //     // precond ends
+    //     AbSeqIndex(AI.AbAdd(i, AI.I1), s) == AbSeqIndex(i, s')
+  // {
+  //   var k := AbSeqGetIdx(v, s);
+  //   AbSeqRemoveIdx(k, s)
+  // }
+  
+  lemma AbSeqInSame_p3<X> (s: AbSeq<X>, s':AbSeq<X>, v: X)
+    requires AbSeqIn(v, s')
+    ensures AbSeqIn(v, s)
 
-  function method AbSeqRemoveIdx<X(!new)> (k: AbInt, s: AbSeq<X>) : (s': AbSeq<X>)
-    requires AbLt(k, AbSeqLen(s))
-    requires AbLt(I0, k) || I0 == k
-    ensures AbSeqLen(s) == AbAdd(AbSeqLen(s'), I1)
-    ensures AbSeqLen(s') == AbSub(AbSeqLen(s), I1)
-    ensures forall v :: AbSeqIn(v, s') ==> AbSeqIn(v, s)
-    ensures
-      forall i :: // s[0, k) keeps
-        AbLeqLt(i, I0, k) ==>
-        // precond begins
-        AbLt(i, AbSeqLen(s)) ==>
-        AbLt(i, AbSeqLen(s')) ==>
-        // precond ends
-        AbSeqIndex(i, s) == AbSeqIndex(i, s')
-    ensures
-      forall i :: // s(k, |s|-1] keeps
-        AbLt(k, i) && AbLt(i, AbSeqLen(s')) ==>
-        // precond begins
-        AbLeq(I0, i) ==>
-        AbLt(I0, AbAdd(i, I1)) ==>
-        AbLt(AbAdd(i, I1), AbSeqLen(s)) ==>
-        // precond ends
-        AbSeqIndex(AbAdd(i, I1), s) == AbSeqIndex(i, s')
-  {
-    var len := AbSeqLen(s);
-    var half1 := AbSeqSlice(I0, k, s);
-    Props_add2sub ();
-    Props_add_identity ();
-    Props_notneg ();
-    assume AbPos(I1); // Props_pos (I1);
-    Props_add_pos_is_lt ();
-    Props_lt_transitive ();
-    if AbLt(AbAdd(k, I1), len) then
-      var half2 := AbSeqSlice(AbAdd(k, I1), len, s);
-      // var s':= AbSeqConcat(half1, half2);
-      Seq_Props_concat_length_p2 (half1, half2);
-      Props_add_associative ();
-      Props_lt_addition ();
-      Seq_Props_concat_index_part1<X> ();
-      // assert forall i :: // s[0, k) keeps
-      //   (AbLt(I0, i) || I0 == i) &&
-      //   AbLt(i, k) ==> 
-      //   AbSeqIndex(i, s) == AbSeqIndex(i, s');
-      Props_add_commutative ();
-      Seq_Props_concat_index_part2<X> ();
-      // assert forall i :: // s(k, |s|-1] keeps
-      //   (AbLt(k, i) || i == k) &&
-      //   AbLt(i, AbSeqLen(s')) ==>
-      //   AbSeqIndex(AbAdd(i, I1), s) == 
-      //   AbSeqIndex(i, s');
-      Seq_Props_slice_in<X> ();
-      Seq_Props_concat_in<X> ();
-      // assert forall v :: AbSeqIn(v, s') ==> AbSeqIn(v, s);
-      AbSeqConcat(half1, half2)
-    else
-      Props_lt_is_not_leq ();
-      Props_lt2leq ();
-      Seq_Props_slice_in<X> ();
-      // assert forall v :: AbSeqIn(v, half1) ==> AbSeqIn(v, s);
-      // assert forall i :: // s[0, k) keeps
-      //   (AbLt(I0, i) || I0 == i) &&
-      //   AbLt(i, AbSub(len, I1)) ==> 
-      //   AbSeqIndex(i, s) == AbSeqIndex(i, s');
-      // assert forall i :: // s(k, |s|-1] keeps
-      //   (AbLt(k, i) || i == k) &&
-      //   AbLt(i, AbSeqLen(s')) ==>
-      //   AbSeqIndex(AbAdd(i, I1), s) == AbSeqIndex(i, s');
-      half1
-  }
+  // s[0, k) keeps
+  lemma AbSeqPart1Same_p4<X>(k: AI.AbInt, s: AbSeq<X>, s': AbSeq<X>, i: AI.AbInt)
+    requires AI.AbLeqLt(i, AI.I0, k)
+    requires AI.AbLt(i, AbSeqLen(s))
+    requires AI.AbLt(i, AbSeqLen(s'))
+    ensures AbSeqIndex(i, s) == AbSeqIndex(i, s')
+  
+  // s[k, |s|-1) shifts
+  lemma AbSeqPart2Shift1_p4<X>(k: AI.AbInt, s: AbSeq<X>, s': AbSeq<X>, i: AI.AbInt)
+    requires AI.AbLeqLt(i, k, AbSeqLen(s'))
+    requires AI.AbLeq(AI.I0, i)
+    requires AI.AbLt(AI.I0, AI.AbAdd(i, AI.I1))
+    requires AI.AbLt(AI.AbAdd(i, AI.I1), AbSeqLen(s))
+    ensures AbSeqIndex(AI.AbAdd(i, AI.I1), s) == AbSeqIndex(i, s')
 
-  function method AbSeqUpdate<X> (k: AbInt, v: X, s: AbSeq<X>): (s': AbSeq<X>)
-    requires AbLt(k, AbSeqLen(s))
-    requires AbLeq(I0, k)
+  function method AbSeqRemoveIdx<X(!new)> (k: AI.AbInt, s: AbSeq<X>) : (s': AbSeq<X>)
+    requires AI.AbLt(k, AbSeqLen(s))
+    requires AI.AbLeq(AI.I0, k)
+    ensures AbSeqLen(s) == AI.AbAdd(AbSeqLen(s'), AI.I1)
+    ensures AbSeqLen(s') == AI.AbSub(AbSeqLen(s), AI.I1)
+    // ensures forall v :: AbSeqIn(v, s') ==> AbSeqIn(v, s)
+    // ensures
+    //   forall i :: // s[0, k) keeps
+    //     AI.AbLeqLt(i, AI.I0, k) ==>
+    //     // precond begins
+    //     AI.AbLt(i, AbSeqLen(s)) ==>
+    //     AI.AbLt(i, AbSeqLen(s')) ==>
+    //     // precond ends
+    //     AbSeqIndex(i, s) == AbSeqIndex(i, s')
+    // ensures
+    //   forall i :: // s[k, |s|-1) keeps
+    //     AI.AbLeqLt(i, k, AbSeqLen(s')) ==>
+    //     // precond begins
+    //     AI.AbLeq(AI.I0, i) ==>
+    //     AI.AbLt(AI.I0, AI.AbAdd(i, AI.I1)) ==>
+    //     AI.AbLt(AI.AbAdd(i, AI.I1), AbSeqLen(s)) ==>
+    //     // precond ends
+    //     AbSeqIndex(AI.AbAdd(i, AI.I1), s) == AbSeqIndex(i, s')
+    { s[ ..k ] + s[ k+1.. ] }
+  // {
+  //   var len := AbSeqLen(s);
+  //   var half1 := AbSeqSlice(AI.I0, k, s);
+  //   Props_add2sub ();
+  //   Props_add_identity ();
+  //   Props_notneg ();
+  //   assume AbPos(AI.I1); // Props_pos (AI.I1);
+  //   Props_add_pos_is_lt ();
+  //   Props_lt_transitive ();
+  //   if AI.AbLt(AI.AbAdd(k, AI.I1), len) then
+  //     var half2 := AbSeqSlice(AI.AbAdd(k, AI.I1), len, s);
+  //     // var s':= AbSeqConcat(half1, half2);
+  //     Seq_Props_concat_length_p2 (half1, half2);
+  //     Props_add_associative ();
+  //     Props_lt_addition ();
+  //     Seq_Props_concat_index_part1<X> ();
+  //     // assert forall i :: // s[0, k) keeps
+  //     //   (AI.AbLt(AI.I0, i) || AI.I0 == i) &&
+  //     //   AI.AbLt(i, k) ==> 
+  //     //   AbSeqIndex(i, s) == AbSeqIndex(i, s');
+  //     Props_add_commutative ();
+  //     Seq_Props_concat_index_part2<X> ();
+  //     // assert forall i :: // s(k, |s|-1] keeps
+  //     //   (AI.AbLt(k, i) || i == k) &&
+  //     //   AI.AbLt(i, AbSeqLen(s')) ==>
+  //     //   AbSeqIndex(AI.AbAdd(i, AI.I1), s) == 
+  //     //   AbSeqIndex(i, s');
+  //     Seq_Props_slice_in<X> ();
+  //     Seq_Props_concat_in<X> ();
+  //     // assert forall v :: AbSeqIn(v, s') ==> AbSeqIn(v, s);
+  //     AbSeqConcat(half1, half2)
+  //   else
+  //     Props_lt_is_not_leq ();
+  //     Props_lt2leq ();
+  //     Seq_Props_slice_in<X> ();
+  //     // assert forall v :: AbSeqIn(v, half1) ==> AbSeqIn(v, s);
+  //     // assert forall i :: // s[0, k) keeps
+  //     //   (AI.AbLt(AI.I0, i) || AI.I0 == i) &&
+  //     //   AI.AbLt(i, AI.AbSub(len, AI.I1)) ==> 
+  //     //   AbSeqIndex(i, s) == AbSeqIndex(i, s');
+  //     // assert forall i :: // s(k, |s|-1] keeps
+  //     //   (AI.AbLt(k, i) || i == k) &&
+  //     //   AI.AbLt(i, AbSeqLen(s')) ==>
+  //     //   AbSeqIndex(AI.AbAdd(i, AI.I1), s) == AbSeqIndex(i, s');
+  //     half1
+  // }
+
+  // s(k, |s|) keeps
+  lemma AbSeqPart2Same_p4<X>(k: AI.AbInt, s: AbSeq<X>, s': AbSeq<X>, i: AI.AbInt)
+    requires AI.AbLt(k, i)
+    requires AI.AbLt(i, AbSeqLen(s'))
+    requires AI.AbLeqLt(i, AI.I0, AbSeqLen(s))
+    ensures AbSeqIndex(i, s) == AbSeqIndex(i, s')
+
+  function method AbSeqUpdate<X> (k: AI.AbInt, v: X, s: AbSeq<X>): (s': AbSeq<X>)
+    requires AI.AbLt(k, AbSeqLen(s))
+    requires AI.AbLeq(AI.I0, k)
     ensures AbSeqLen(s) == AbSeqLen(s')
     ensures AbSeqIndex(k, s') == v
-    ensures
-      forall i :: // s[0, k) keeps
-        AbLeqLt(i, I0, k) ==>
-        // precond begins
-        AbLt(i, AbSeqLen(s)) ==>
-        AbLt(i, AbSeqLen(s')) ==>
-        // precond ends
-        AbSeqIndex(i, s) == AbSeqIndex(i, s')
-    ensures
-      forall i :: // s(k, |s|-1] keeps
-        AbLt(k, i) && AbLt(i, AbSeqLen(s')) ==>
-        // precond begins
-        AbLeq(I0, i) ==>
-        AbLt(i, AbSeqLen(s)) ==>
-        // precond ends
-        AbSeqIndex(i, s) == AbSeqIndex(i, s')
-  {
-    var len := AbSeqLen(s);
-    var half1 := AbSeqSlice(I0, k, s);
-    Props_add2sub ();
-    Props_add_identity ();
-    Props_notneg ();
-    assume AbPos(I1); // Props_pos (I1);
-    Props_add_pos_is_lt ();
-    Props_lt_transitive ();
-    Props_add_commutative ();
-    if AbLt(AbAdd(k, I1), len) then
-      var half2 := AbSeqSlice(AbAdd(k, I1), len, s);
-      var half1' := AbSeqConcat(half1, AbSeqSingleton(v));
-      Seq_Props_concat_length_p2 (half1, AbSeqSingleton(v));
-      Seq_Props_concat_length_p2 (half1', half2);
-      // var s' := AbSeqConcat(half1', half2);
-      // assert len == AbSeqLen(s');
-      Props_lt_addition ();
-      Seq_Props_concat_index_part1<X> ();
-      // assert forall i :: // s[0, k) keeps
-      //   (AbLt(I0, i) || I0 == i) &&
-      //   AbLt(i, k) ==>
-      //   AbSeqIndex(i, s) == AbSeqIndex(i, s');
-      // Seq_Props_concat_is_orig<X> ();
-      Seq_Props_concat_is_orig_p2 (AbAdd(k, I1), s);
-      Seq_Props_concat_index_part2<X> ();
-      // Seq_Props_concat_index_part2_param (I0, half1, AbSeqSingleton(v));
-      // assert AbSeqIndex(k, half1') == v;
+    // ensures
+    //   forall i :: // s[0, k) keeps
+    //     AI.AbLeqLt(i, AI.I0, k) ==>
+    //     // precond begins
+    //     AI.AbLt(i, AbSeqLen(s)) ==>
+    //     AI.AbLt(i, AbSeqLen(s')) ==>
+    //     // precond ends
+    //     AbSeqIndex(i, s) == AbSeqIndex(i, s')
+    // ensures
+    //   forall i :: // s(k, |s|) keeps
+    //     AI.AbLt(k, i) && AI.AbLt(i, AbSeqLen(s')) ==>
+    //     // precond begins
+    //     AI.AbLeq(AI.I0, i) ==>
+    //     AI.AbLt(i, AbSeqLen(s)) ==>
+    //     // precond ends
+    //     AbSeqIndex(i, s) == AbSeqIndex(i, s')
+    { s[ k := v ] }
+  // {
+  //   var len := AbSeqLen(s);
+  //   var half1 := AbSeqSlice(AI.I0, k, s);
+  //   Props_add2sub ();
+  //   Props_add_identity ();
+  //   Props_notneg ();
+  //   assume AbPos(AI.I1); // Props_pos (AI.I1);
+  //   Props_add_pos_is_lt ();
+  //   Props_lt_transitive ();
+  //   Props_add_commutative ();
+  //   if AI.AbLt(AI.AbAdd(k, AI.I1), len) then
+  //     var half2 := AbSeqSlice(AI.AbAdd(k, AI.I1), len, s);
+  //     var half1' := AbSeqConcat(half1, AbSeqSingleton(v));
+  //     Seq_Props_concat_length_p2 (half1, AbSeqSingleton(v));
+  //     Seq_Props_concat_length_p2 (half1', half2);
+  //     // var s' := AbSeqConcat(half1', half2);
+  //     // assert len == AbSeqLen(s');
+  //     Props_lt_addition ();
+  //     Seq_Props_concat_index_part1<X> ();
+  //     // assert forall i :: // s[0, k) keeps
+  //     //   (AI.AbLt(AI.I0, i) || AI.I0 == i) &&
+  //     //   AI.AbLt(i, k) ==>
+  //     //   AbSeqIndex(i, s) == AbSeqIndex(i, s');
+  //     // Seq_Props_concat_is_orig<X> ();
+  //     Seq_Props_concat_is_orig_p2 (AI.AbAdd(k, AI.I1), s);
+  //     Seq_Props_concat_index_part2<X> ();
+  //     // Seq_Props_concat_index_part2_param (AI.I0, half1, AbSeqSingleton(v));
+  //     // assert AbSeqIndex(k, half1') == v;
       
-      // assert forall i :: // s(k, |s|-1] keeps
-      //   AbLt(k, i) && AbLt(i, AbSeqLen(s)) ==>
-      //   AbSeqIndex(i, s) == AbSeqIndex(AbSub(i, AbAdd(k, I1)), half2);
-      // assert forall i :: // s(k, |s|-1] keeps
-      //   AbLt(k, i) &&
-      //   AbLt(i, AbSeqLen(s')) ==>
-      //   AbSeqIndex(i, s) == AbSeqIndex(i, s');
-      AbSeqConcat(half1', half2)
-    else
-      Props_lt_is_not_leq_p2 (AbAdd(k, I1), len);
-      Props_lt2leq ();
-      // var s' := AbSeqConcat(half1, AbSeqSingleton(v));
-      Seq_Props_concat_length_p2 (half1, AbSeqSingleton(v));
-      // assert AbSeqLen(s') == len;
-      Seq_Props_concat_index_part1<X> ();
-      // assert forall i :: // s[0, k) keeps
-      //   (AbLt(I0, i) || I0 == i) &&
-      //   AbLt(i, k) ==>
-      //   AbSeqIndex(i, s) == AbSeqIndex(i, s');
-      // assert forall i :: // s(k, |s|-1] keeps
-      //   AbLt(k, i) &&
-      //   AbLt(i, AbSeqLen(s')) ==>
-      //   AbSeqIndex(i, s) == AbSeqIndex(i, s');
-      Seq_Props_concat_index_part2<X> ();
-      // assert AbSeqIndex(k, s') == v;
-      AbSeqConcat(half1, AbSeqSingleton(v))
-}
+  //     // assert forall i :: // s(k, |s|-1] keeps
+  //     //   AI.AbLt(k, i) && AI.AbLt(i, AbSeqLen(s)) ==>
+  //     //   AbSeqIndex(i, s) == AbSeqIndex(AI.AbSub(i, AI.AbAdd(k, AI.I1)), half2);
+  //     // assert forall i :: // s(k, |s|-1] keeps
+  //     //   AI.AbLt(k, i) &&
+  //     //   AI.AbLt(i, AbSeqLen(s')) ==>
+  //     //   AbSeqIndex(i, s) == AbSeqIndex(i, s');
+  //     AbSeqConcat(half1', half2)
+  //   else
+  //     Props_lt_is_not_leq_p2 (AI.AbAdd(k, AI.I1), len);
+  //     Props_lt2leq ();
+  //     // var s' := AbSeqConcat(half1, AbSeqSingleton(v));
+  //     Seq_Props_concat_length_p2 (half1, AbSeqSingleton(v));
+  //     // assert AbSeqLen(s') == len;
+  //     Seq_Props_concat_index_part1<X> ();
+  //     // assert forall i :: // s[0, k) keeps
+  //     //   (AI.AbLt(AI.I0, i) || AI.I0 == i) &&
+  //     //   AI.AbLt(i, k) ==>
+  //     //   AbSeqIndex(i, s) == AbSeqIndex(i, s');
+  //     // assert forall i :: // s(k, |s|-1] keeps
+  //     //   AI.AbLt(k, i) &&
+  //     //   AI.AbLt(i, AbSeqLen(s')) ==>
+  //     //   AbSeqIndex(i, s) == AbSeqIndex(i, s');
+  //     Seq_Props_concat_index_part2<X> ();
+  //     // assert AbSeqIndex(k, s') == v;
+  //     AbSeqConcat(half1, AbSeqSingleton(v))
+  //  }
 
   lemma Seq_Props_length_p1<X> (s: AbSeq<X>) // |s| >= 0
-    ensures forall s: AbSeq<X> :: AbLeq(I0, AbSeqLen(s))
-    {}
-  lemma Seq_Props_length<X> () // |s| >= 0
-    ensures forall s: AbSeq<X> :: AbLeq(I0, AbSeqLen(s))
-    { forall s { Seq_Props_length_p1<X> (s); } }
+    ensures AI.AbLeq(AI.I0, AbSeqLen(s))
+    { }
 
   lemma Seq_Props_concat_length_p2<X> (s1: AbSeq<X>, s2: AbSeq<X>) // |s1 + s2| == |s1| + |s2|
-    ensures AbSeqLen(AbSeqConcat(s1, s2)) == AbAdd(AbSeqLen(s1), AbSeqLen(s2))
+    ensures AbSeqLen(AbSeqConcat(s1, s2)) == AI.AbAdd(AbSeqLen(s1), AbSeqLen(s2))
     { }
-  lemma Seq_Props_concat_length<X> () // |s1 + s2| == |s1| + |s2|
-    ensures forall s1: AbSeq<X>, s2: AbSeq<X> :: AbSeqLen(AbSeqConcat(s1, s2)) == AbAdd(AbSeqLen(s1), AbSeqLen(s2))
-    { forall s1, s2 { Seq_Props_concat_length_p2<X>(s1, s2); } }
   
-  lemma Seq_Props_concat_in_p3<X> (x: X, s1: AbSeq<X>, s2: AbSeq<X>) // x in s1 || x in s2 <==> x in s1 + s2
-    ensures AbSeqIn(x, s1) || AbSeqIn(x, s2) <==> AbSeqIn(x, AbSeqConcat(s1, s2))
+  lemma Seq_Props_concat_in_p3<X> (x: X, s1: AbSeq<X>, s2: AbSeq<X>) // x in s1 || x in s2 ==> x in s1 + s2
+    requires AbSeqIn(x, s1) || AbSeqIn(x, s2)
+    ensures AbSeqIn(x, AbSeqConcat(s1, s2))
     { }
-  lemma Seq_Props_concat_in<X> () // x in s1 || x in s2 <==> x in s1 + s2
-    ensures forall x: X, s1: AbSeq<X>, s2: AbSeq<X> :: AbSeqIn(x, s1) || AbSeqIn(x, s2) <==> AbSeqIn(x, AbSeqConcat(s1, s2))
-    { forall x, s1, s2 { Seq_Props_concat_in_p3<X>(x, s1, s2); } }
 
-  lemma Seq_Props_concat_in_part2all_p3<X> (x: X, s1: AbSeq<X>, s2: AbSeq<X>)
+  lemma Seq_Props_concat_in_part1_all_p3<X> (x: X, s1: AbSeq<X>, s2: AbSeq<X>)
     // x in s1 ==> x in s1 + s2
-    ensures AbSeqIn(x, s1) ==> AbSeqIn(x, AbSeqConcat(s1, s2))
+    requires AbSeqIn(x, s1)
+    ensures AbSeqIn(x, AbSeqConcat(s1, s2))
+  
+  lemma Seq_Props_concat_in_part2_all_p3<X> (x: X, s1: AbSeq<X>, s2: AbSeq<X>)
     // x in s2 ==> x in s1 + s2
-    ensures AbSeqIn(x, s2) ==> AbSeqIn(x, AbSeqConcat(s1, s2))
+    requires AbSeqIn(x, s2)
+    ensures AbSeqIn(x, AbSeqConcat(s1, s2))
     { }
-  lemma Seq_Props_concat_in_part2all<X> ()
-    // x in s1 ==> x in s1 + s2
-    ensures forall x: X, s1: AbSeq<X>, s2: AbSeq<X> :: AbSeqIn(x, s1) ==> AbSeqIn(x, AbSeqConcat(s1, s2))
-    // x in s2 ==> x in s1 + s2
-    ensures forall x: X, s1: AbSeq<X>, s2: AbSeq<X> :: AbSeqIn(x, s2) ==> AbSeqIn(x, AbSeqConcat(s1, s2))
-    { forall x, s1, s2 { Seq_Props_concat_in_part2all_p3<X>(x, s1, s2); } }
 
-  lemma Seq_Props_concat_in_all2part_p3<X> (x: X, s1: AbSeq<X>, s2: AbSeq<X>)
-    // x in s1 + s2 && x !in s1 ==> x in s2
-    ensures AbSeqIn(x, AbSeqConcat(s1, s2)) && !AbSeqIn(x, s1) ==> AbSeqIn(x, s2)
+  lemma Seq_Props_concat_in_all_part1_p3<X> (x: X, s1: AbSeq<X>, s2: AbSeq<X>)
     // x in s1 + s2 && x !in s2 ==> x in s1
-    ensures AbSeqIn(x, AbSeqConcat(s1, s2)) && !AbSeqIn(x, s2) ==> AbSeqIn(x, s1)
+    requires AbSeqIn(x, AbSeqConcat(s1, s2))
+    requires !AbSeqIn(x, s2)
+    ensures AbSeqIn(x, s1)
     { }
-  lemma Seq_Props_concat_in_all2part<X> ()
+
+  lemma Seq_Props_concat_in_all_part2_p3<X> (x: X, s1: AbSeq<X>, s2: AbSeq<X>)
     // x in s1 + s2 && x !in s1 ==> x in s2
-    ensures forall x: X, s1: AbSeq<X>, s2: AbSeq<X> :: AbSeqIn(x, AbSeqConcat(s1, s2)) && !AbSeqIn(x, s1) ==> AbSeqIn(x, s2)
-    // x in s1 + s2 && x !in s2 ==> x in s1
-    ensures forall x: X, s1: AbSeq<X>, s2: AbSeq<X> :: AbSeqIn(x, AbSeqConcat(s1, s2)) && !AbSeqIn(x, s2) ==> AbSeqIn(x, s1)
-    { forall x, s1, s2 { Seq_Props_concat_in_all2part_p3<X>(x, s1, s2); } }
-
-  lemma Seq_Props_concat_index_part1_p3<X> (i: AbInt, s1: AbSeq<X>, s2: AbSeq<X>)
-    ensures AbLeqLt(i, I0, AbSeqLen(s1)) ==> // 0 <= i < |s1|
-    AbLt(i, AbSeqLen(AbSeqConcat(s1, s2))) ==> // i < |s1| < |s1 + s2|
-    AbSeqIndex(i, s1) == AbSeqIndex(i, AbSeqConcat(s1, s2))
+    requires AbSeqIn(x, AbSeqConcat(s1, s2))
+    requires !AbSeqIn(x, s1)
+    ensures AbSeqIn(x, s2)
     { }
-  lemma Seq_Props_concat_index_part1<X> ()
-    ensures forall i: AbInt, s1: AbSeq<X>, s2: AbSeq<X> ::
-    AbLeqLt(i, I0, AbSeqLen(s1)) ==> // 0 <= i < |s1|
-    AbLt(i, AbSeqLen(AbSeqConcat(s1, s2))) ==> // i < |s1| < |s1 + s2|
-    AbSeqIndex(i, s1) == AbSeqIndex(i, AbSeqConcat(s1, s2))
-    { forall i, s1, s2 { Seq_Props_concat_index_part1_p3<X>(i, s1, s2); } }
 
-  lemma Seq_Props_concat_index_part2_p3<X> (i: AbInt, s1: AbSeq<X>, s2: AbSeq<X>)
-    ensures AbLeq(I0, AbAdd(i, AbSeqLen(s1))) ==> // 0 <= i + |s1|
-      (AbLt(i, AbSeqLen(s2)) ==> AbLt(AbAdd(i, AbSeqLen(s1)), AbSeqLen(AbSeqConcat(s1, s2)))) ==> // i + |s1| < |s1 + s2|
-      AbLeqLt(i, I0, AbSeqLen(s2)) ==>
-      AbSeqIndex(i, s2) == AbSeqIndex(AbAdd(i, AbSeqLen(s1)), AbSeqConcat(s1, s2))
+  lemma Seq_Props_concat_index_part1_p3<X> (i: AI.AbInt, s1: AbSeq<X>, s2: AbSeq<X>)
+    requires AI.AbLeqLt(i, AI.I0, AbSeqLen(s1)) // 0 <= i < |s1|
+    requires AI.AbLt(i, AbSeqLen(AbSeqConcat(s1, s2))) // i < |s1| < |s1 + s2|
+    ensures AbSeqIndex(i, s1) == AbSeqIndex(i, AbSeqConcat(s1, s2))
     { }
-  lemma Seq_Props_concat_index_part2<X> ()
-    ensures forall i: AbInt, s1: AbSeq<X>, s2: AbSeq<X> ::
-      AbLeq(I0, AbAdd(i, AbSeqLen(s1))) ==> // 0 <= i + |s1|
-      (AbLt(i, AbSeqLen(s2)) ==> AbLt(AbAdd(i, AbSeqLen(s1)), AbSeqLen(AbSeqConcat(s1, s2)))) ==> // i + |s1| < |s1 + s2|
-      AbLeqLt(i, I0, AbSeqLen(s2)) ==>
-      AbSeqIndex(i, s2) == AbSeqIndex(AbAdd(i, AbSeqLen(s1)), AbSeqConcat(s1, s2))
-    { forall i, s1, s2 { Seq_Props_concat_index_part2_p3<X>(i, s1, s2); } }
 
-  lemma Seq_Props_concat_is_orig_p2<X> (i: AbInt, s: AbSeq<X>)
-    ensures AbLeqLt(i, I0, AbSeqLen(s)) ==> // 0 <= i < |s|
-      s == AbSeqConcat(AbSeqSlice(I0, i, s), AbSeqSlice(i, AbSeqLen(s), s))
+  lemma Seq_Props_concat_index_part2_p3<X> (i: AI.AbInt, s1: AbSeq<X>, s2: AbSeq<X>)
+    requires AI.AbLeqLt(i, AI.I0, AbSeqLen(s2)) // 0 <= i < |s2|
+    requires AI.AbLeq(AI.I0, AI.AbAdd(i, AbSeqLen(s1))) // 0 <= i + |s1|
+    requires AI.AbLt(AI.AbAdd(i, AbSeqLen(s1)), AbSeqLen(AbSeqConcat(s1, s2)))  // i + |s1| < |s1 + s2|
+    ensures AbSeqIndex(i, s2) == AbSeqIndex(AI.AbAdd(i, AbSeqLen(s1)), AbSeqConcat(s1, s2))
     { }
-  lemma Seq_Props_concat_is_orig<X> ()
-    ensures forall i: AbInt, s: AbSeq<X> ::
-      AbLeqLt(i, I0, AbSeqLen(s)) ==> // 0 <= i < |s|
-      s == AbSeqConcat(AbSeqSlice(I0, i, s), AbSeqSlice(i, AbSeqLen(s), s))
-    { forall i, s { Seq_Props_concat_is_orig_p2<X> (i, s); } }
+
+  lemma Seq_Props_concat_is_orig_p2<X> (i: AI.AbInt, s: AbSeq<X>)
+    requires AI.AbLeqLt(i, AI.I0, AbSeqLen(s)) // 0 <= i < |s|
+    ensures s == AbSeqConcat(AbSeqSlice(AI.I0, i, s), AbSeqSlice(i, AbSeqLen(s), s))
+    { }
 
   lemma Seq_Props_in_empty_p2<X> (v: X, s: AbSeq<X>) // empty seq
-    ensures AbSeqLen(s) == I0 ==> !AbSeqIn(v, s)
+    requires AbSeqLen(s) == AI.I0
+    ensures !AbSeqIn(v, s)
     { }
-  lemma Seq_Props_in_empty<X> () // empty seq
-    ensures forall v: X, s: AbSeq<X> :: AbSeqLen(s) == I0 ==> !AbSeqIn(v, s)
-    {forall v, s { Seq_Props_in_empty_p2<X>(v, s); } }
 
   lemma Seq_Props_in_non_empty_p2<X> (v: X, s: AbSeq<X>) // i in s ==> |s| > 0
-    ensures AbSeqIn(v, s) ==> AbLt(I0, AbSeqLen(s))
+    requires AbSeqIn(v, s)
+    ensures AI.AbLt(AI.I0, AbSeqLen(s))
     { }
-  lemma Seq_Props_in_non_empty<X> () // i in s ==> |s| > 0
-    ensures forall v: X, s: AbSeq<X> :: AbSeqIn(v, s) ==> AbLt(I0, AbSeqLen(s))
-    {forall v, s { Seq_Props_in_non_empty_p2<X>(v, s); } }
 
   lemma Seq_Props_in_idx_p2<X> (v: X, s: AbSeq<X>) // v in s ==> s[i] == v
-    ensures AbSeqIn(v, s) ==>
-      (exists i: AbInt :: AbLeqLt(i, I0, AbSeqLen(s)) && AbSeqIndex(i, s) == v )
-  // NOTE: NEED PROVE
-  lemma Seq_Props_in_idx<X> () // v in s ==> s[i] == v
-    ensures forall v: X, s: AbSeq<X> :: AbSeqIn(v, s) ==>
-      (exists i: AbInt :: AbLeqLt(i, I0, AbSeqLen(s)) && AbSeqIndex(i, s) == v )
-    { forall v, s { Seq_Props_in_idx_p2<X>(v, s); } }
+    requires AbSeqIn(v, s)
+    ensures exists i: AI.AbInt :: AI.AbLeqLt(i, AI.I0, AbSeqLen(s)) && AbSeqIndex(i, s) == v
+    // { ghost var k :| 0 <= k < |s| && s[k] == v; if exists i : AI.AbInt :: i == k { } }
+    // TODO
 
-  lemma Seq_Props_slice_in_p4<X> (i: AbInt, j: AbInt, s: AbSeq<X>, v: X)
-    ensures AbLeq(I0, i) && AbLeq(j, AbSeqLen(s)) && AbLeq(i, j) ==>
-      AbSeqIn(v, AbSeqSlice(i, j, s)) ==> AbSeqIn(v, s)
+  lemma Seq_Props_slice_in_p4<X> (i: AI.AbInt, j: AI.AbInt, s: AbSeq<X>, v: X)
+    requires AI.AbLeq(AI.I0, i) 
+    requires AI.AbLeq(j, AbSeqLen(s))
+    requires AI.AbLeq(i, j)
+    ensures AbSeqIn(v, AbSeqSlice(i, j, s)) ==> AbSeqIn(v, s)
     { }
-  lemma Seq_Props_slice_in<X> ()
-    ensures forall i: AbInt, j: AbInt, s: AbSeq<X>, v: X ::
-      AbLeq(I0, i) && AbLeq(j, AbSeqLen(s)) && AbLeq(i, j) ==>
-      AbSeqIn(v, AbSeqSlice(i, j, s)) ==> AbSeqIn(v, s)
-    { forall i, j, s, v { Seq_Props_slice_in_p4<X>(i, j, s, v); } }
 
+  lemma Seq_Props_index_props_lt (i: AI.AbInt, j: AI.AbInt, x: AI.AbInt, s: AbSeq<AI.AbInt>, s': AbSeq<AI.AbInt>)
+    requires AI.AbLeqLt(i, AI.I0, AbSeqLen(s))
+    requires AI.AbLeqLt(j, AI.I0, AbSeqLen(s'))
+    // requires forall v :: AbSeqIn(v, s') ==> AbSeqIn(v, s)
+    requires AbSeqIn(AbSeqIndex(j, s'), s)
+    requires AI.AbLt(AbSeqIndex(i, s), x)
+    ensures AI.AbLt(AbSeqIndex(j, s'), x)
+    { }
+
+  lemma Seq_Props_index_props_gt (i: AI.AbInt, j: AI.AbInt, x: AI.AbInt, s: AbSeq<AI.AbInt>, s': AbSeq<AI.AbInt>)
+    requires AI.AbLeqLt(i, AI.I0, AbSeqLen(s))
+    requires AI.AbLeqLt(j, AI.I0, AbSeqLen(s'))
+    // requires forall v :: AbSeqIn(v, s') ==> AbSeqIn(v, s)
+    requires AbSeqIn(AbSeqIndex(j, s'), s)
+    requires AI.AbLt(x, AbSeqIndex(i, s))
+    ensures AI.AbLt(x, AbSeqIndex(j, s'))
+    { }
 }
 
-module ADT_SeqLemma {
-  import opened ADT_Seq`Basic
+import opened ADT`Basic
+import opened ADT_Seq`Seq_Basic
 
-  lemma Seq_Props_length<X> () // |s| >= 0
-    ensures forall s: AbSeq<X> :: AbLeq(I0, AbSeqLen(s))
-    { forall s { Seq_Props_length_p1<X> (s); } }
-  
-  lemma Seq_Props_concat_length<X> () // |s1 + s2| == |s1| + |s2|
-    ensures forall s1: AbSeq<X>, s2: AbSeq<X> :: AbSeqLen(AbSeqConcat(s1, s2)) == AbAdd(AbSeqLen(s1), AbSeqLen(s2))
-    { forall s1, s2 { Seq_Props_concat_length_p2<X>(s1, s2); } }
-  
-  lemma Seq_Props_concat_in<X> () // x in s1 || x in s2 <==> x in s1 + s2
-    ensures forall x: X, s1: AbSeq<X>, s2: AbSeq<X> :: AbSeqIn(x, s1) || AbSeqIn(x, s2) <==> AbSeqIn(x, AbSeqConcat(s1, s2))
-    { forall x, s1, s2 { Seq_Props_concat_in_p3<X>(x, s1, s2); } }
-  
-  lemma Seq_Props_concat_in_part2all<X> ()
-    // x in s1 ==> x in s1 + s2
-    ensures forall x: X, s1: AbSeq<X>, s2: AbSeq<X> :: AbSeqIn(x, s1) ==> AbSeqIn(x, AbSeqConcat(s1, s2))
-    // x in s2 ==> x in s1 + s2
-    ensures forall x: X, s1: AbSeq<X>, s2: AbSeq<X> :: AbSeqIn(x, s2) ==> AbSeqIn(x, AbSeqConcat(s1, s2))
-    { forall x, s1, s2 { Seq_Props_concat_in_part2all_p3<X>(x, s1, s2); } }
-  
-  lemma Seq_Props_concat_in_all2part<X> ()
-    // x in s1 + s2 && x !in s1 ==> x in s2
-    ensures forall x: X, s1: AbSeq<X>, s2: AbSeq<X> :: AbSeqIn(x, AbSeqConcat(s1, s2)) && !AbSeqIn(x, s1) ==> AbSeqIn(x, s2)
-    // x in s1 + s2 && x !in s2 ==> x in s1
-    ensures forall x: X, s1: AbSeq<X>, s2: AbSeq<X> :: AbSeqIn(x, AbSeqConcat(s1, s2)) && !AbSeqIn(x, s2) ==> AbSeqIn(x, s1)
-    { forall x, s1, s2 { Seq_Props_concat_in_all2part_p3<X>(x, s1, s2); } }
-  
-  lemma Seq_Props_concat_index_part1<X> ()
-    ensures forall i: AbInt, s1: AbSeq<X>, s2: AbSeq<X> ::
-    AbLeqLt(i, I0, AbSeqLen(s1)) ==> // 0 <= i < |s1|
-    AbLt(i, AbSeqLen(AbSeqConcat(s1, s2))) ==> // i < |s1| < |s1 + s2|
-    AbSeqIndex(i, s1) == AbSeqIndex(i, AbSeqConcat(s1, s2))
-    { forall i, s1, s2 { Seq_Props_concat_index_part1_p3<X>(i, s1, s2); } }
-  
-  lemma Seq_Props_concat_index_part2<X> ()
-    ensures forall i: AbInt, s1: AbSeq<X>, s2: AbSeq<X> ::
-      AbLeq(I0, AbAdd(i, AbSeqLen(s1))) ==> // 0 <= i + |s1|
-      (AbLt(i, AbSeqLen(s2)) ==> AbLt(AbAdd(i, AbSeqLen(s1)), AbSeqLen(AbSeqConcat(s1, s2)))) ==> // i + |s1| < |s1 + s2|
-      AbLeqLt(i, I0, AbSeqLen(s2)) ==>
-      AbSeqIndex(i, s2) == AbSeqIndex(AbAdd(i, AbSeqLen(s1)), AbSeqConcat(s1, s2))
-    { forall i, s1, s2 { Seq_Props_concat_index_part2_p3<X>(i, s1, s2); } }
-  
-  lemma Seq_Props_concat_is_orig<X> ()
-    ensures forall i: AbInt, s: AbSeq<X> ::
-      AbLeqLt(i, I0, AbSeqLen(s)) ==> // 0 <= i < |s|
-      s == AbSeqConcat(AbSeqSlice(I0, i, s), AbSeqSlice(i, AbSeqLen(s), s))
-    { forall i, s { Seq_Props_concat_is_orig_p2<X> (i, s); } }
-  
-  lemma Seq_Props_in_empty<X> () // empty seq
-    ensures forall v: X, s: AbSeq<X> :: AbSeqLen(s) == I0 ==> !AbSeqIn(v, s)
-    {forall v, s { Seq_Props_in_empty_p2<X>(v, s); } }
-  
-  lemma Seq_Props_in_non_empty<X> () // i in s ==> |s| > 0
-    ensures forall v: X, s: AbSeq<X> :: AbSeqIn(v, s) ==> AbLt(I0, AbSeqLen(s))
-    {forall v, s { Seq_Props_in_non_empty_p2<X>(v, s); } }
-  
-  lemma Seq_Props_in_idx<X> () // v in s ==> s[i] == v
-    ensures forall v: X, s: AbSeq<X> :: AbSeqIn(v, s) ==>
-      (exists i: AbInt :: AbLeqLt(i, I0, AbSeqLen(s)) && AbSeqIndex(i, s) == v )
-    { forall v, s { Seq_Props_in_idx_p2<X>(v, s); } }
-  
-  lemma Seq_Props_slice_in<X> ()
-    ensures forall i: AbInt, j: AbInt, s: AbSeq<X>, v: X ::
-      AbLeq(I0, i) && AbLeq(j, AbSeqLen(s)) && AbLeq(i, j) ==>
-      AbSeqIn(v, AbSeqSlice(i, j, s)) ==> AbSeqIn(v, s)
-    { forall i, j, s, v { Seq_Props_slice_in_p4<X>(i, j, s, v); } }
-}
+// lemma AbSeqInitFunc_p4<X> (len: AI.AbInt, func : AI.AbInt --> X, s: AbSeq<X>, k: AI.AbInt)
+//   requires AI.AbLeqLt(k, AI.I0, len)
+//   requires func.requires(k)
+//   requires AbSeqLen(s) == len // |s| == len, 0 <= k < |s|
+//   ensures AbSeqIndex(k, s) == func(k)
+
+// lemma AbSeqInitFunc<X> (len: AbInt, func : AbInt --> X, s: AbSeq<X>)
+//   requires forall i :: AbLeqLt(i, I0, len) ==> func.requires(i)
+//   requires AbSeqLen(s) == len // |s| == len, 0 <= k < |s|
+//   ensures forall k :: AbLeqLt(k, I0, len) ==> AbSeqIndex(k, s) == func(k)
+//   { forall k | AbLeqLt(k, I0, len)
+//     { AbSeqInitFunc_p4(len, func, s, k); } }
+
+function method AbSeqInit<X> (len: AbInt, func : AbInt --> X) : (s: AbSeq<X>)
+  requires AbLeq(I0, len)
+  requires forall i :: AbLeqLt(i, I0, len) ==> func.requires(i)
+  ensures AbSeqLen(s) == len
+  ensures forall i :: AbLeqLt(i, I0, len) ==> AbSeqIndex(i, s) == func(i)
+
+lemma AbSeqSliceSame<X> (i: AbInt, j: AbInt, s: AbSeq<X>, s': AbSeq<X>)
+  requires AbLeq(I0, i)
+  requires AbLeq(j, AbSeqLen(s))
+  requires AbLeq(i, j)
+  requires AbSeqLen(s') == AbSub(j, i) // |s'| == j-i
+  ensures forall k ::
+    AbLeqLt(k, i, j) && 
+    AbLeqLt(k, I0, AbSeqLen(s)) && // 0 <= k <= s
+    AbLeqLt(AbSub(k, i), I0, AbSeqLen(s')) // 0 <= k-i <= |s'|
+    ==> AbSeqIndex(k, s) == AbSeqIndex(AbSub(k, i), s')
+  { forall k | AbLeqLt(k, i, j) && 
+    AbLeqLt(k, I0, AbSeqLen(s)) && // 0 <= k <= s
+    AbLeqLt(AbSub(k, i), I0, AbSeqLen(s')) // 0 <= k-i <= |s'|
+    { AbSeqSliceSame_p5(i, j, s, s', k); } }
+
+
+lemma AbSeqInSame<X> (s: AbSeq<X>, s':AbSeq<X>)
+  ensures forall v :: AbSeqIn(v, s') ==> AbSeqIn(v, s)
+  { forall v | AbSeqIn(v, s')
+    {AbSeqInSame_p3(s, s', v); } }
+
+lemma AbSeqPart1Same<X>(k: AbInt, s: AbSeq<X>, s': AbSeq<X>)
+  // s[0, k) keeps
+  ensures forall i :: AbLeqLt(i, I0, k) && 
+    AbLt(i, AbSeqLen(s)) && AbLt(i, AbSeqLen(s'))
+     ==> AbSeqIndex(i, s) == AbSeqIndex(i, s')
+  { forall i | AbLeqLt(i, I0, k) && 
+    AbLt(i, AbSeqLen(s)) && AbLt(i, AbSeqLen(s'))
+    { AbSeqPart1Same_p4(k, s, s', i); } }
+
+lemma AbSeqPart2Same<X>(k: AbInt, s: AbSeq<X>, s': AbSeq<X>)
+  // s(k, |s|) keeps
+  ensures forall i :: AbLt(k, i) && AbLt(i, AbSeqLen(s')) && 
+    AbLeqLt(i, I0, AbSeqLen(s))
+    ==> AbSeqIndex(i, s) == AbSeqIndex(i, s')
+  { forall i | AbLt(k, i) && AbLt(i, AbSeqLen(s')) && 
+    AbLeqLt(i, I0, AbSeqLen(s))
+    { AbSeqPart2Same_p4(k, s, s', i); } }
+
+lemma AbSeqPart2Shift1<X>(k: AbInt, s: AbSeq<X>, s': AbSeq<X>)
+  // s[k, |s|-1) shifts
+  ensures forall i :: AbLeqLt(i, k, AbSeqLen(s')) && AbLeq(I0, i) &&
+    AbLt(I0, AbAdd(i, I1)) && AbLt(AbAdd(i, I1), AbSeqLen(s))
+    ==> AbSeqIndex(AbAdd(i, I1), s) == AbSeqIndex(i, s')
+  { forall i | AbLeqLt(i, k, AbSeqLen(s')) && AbLeq(I0, i) &&
+    AbLt(I0, AbAdd(i, I1)) && AbLt(AbAdd(i, I1), AbSeqLen(s))
+    { AbSeqPart2Shift1_p4(k, s, s', i); } }
+
+lemma Seq_Props_length<X> () // |s| >= 0
+  ensures forall s: AbSeq<X> :: AbLeq(I0, AbSeqLen(s))
+  { forall s { Seq_Props_length_p1<X> (s); } }
+
+lemma Seq_Props_concat_length<X> () // |s1 + s2| == |s1| + |s2|
+  ensures forall s1: AbSeq<X>, s2: AbSeq<X> :: AbSeqLen(AbSeqConcat(s1, s2)) == AbAdd(AbSeqLen(s1), AbSeqLen(s2))
+  { forall s1, s2 { Seq_Props_concat_length_p2<X>(s1, s2); } }
+
+lemma Seq_Props_concat_in<X> () // x in s1 || x in s2 ==> x in s1 + s2
+  ensures forall x: X, s1: AbSeq<X>, s2: AbSeq<X> :: AbSeqIn(x, s1) || AbSeqIn(x, s2) ==> AbSeqIn(x, AbSeqConcat(s1, s2))
+  { forall x, s1, s2 | AbSeqIn(x, s1) || AbSeqIn(x, s2)
+    { Seq_Props_concat_in_p3<X>(x, s1, s2); } }
+
+lemma Seq_Props_concat_in_part1_all<X> ()
+  // x in s1 ==> x in s1 + s2
+  ensures forall x: X, s1: AbSeq<X>, s2: AbSeq<X> :: AbSeqIn(x, s1) ==> AbSeqIn(x, AbSeqConcat(s1, s2))
+  { forall x, s1, s2 | AbSeqIn (x, s1) 
+    { Seq_Props_concat_in_part1_all_p3<X>(x, s1, s2); } }
+
+lemma Seq_Props_concat_in_part2_all<X> ()
+  // x in s2 ==> x in s1 + s2
+  ensures forall x: X, s1: AbSeq<X>, s2: AbSeq<X> :: AbSeqIn(x, s2) ==> AbSeqIn(x, AbSeqConcat(s1, s2))
+  { forall x, s1, s2 | AbSeqIn (x, s2) 
+    { Seq_Props_concat_in_part2_all_p3<X>(x, s1, s2); } }
+
+lemma Seq_Props_concat_in_all_part1<X> ()
+  // x in s1 + s2 && x !in s2 ==> x in s1
+  ensures forall x: X, s1: AbSeq<X>, s2: AbSeq<X> :: AbSeqIn(x, AbSeqConcat(s1, s2)) && !AbSeqIn(x, s2) ==> AbSeqIn(x, s1)
+  { forall x, s1, s2 | AbSeqIn(x, AbSeqConcat(s1, s2)) && !AbSeqIn(x, s2)
+    { Seq_Props_concat_in_all_part1_p3<X>(x, s1, s2); } }
+
+lemma Seq_Props_concat_in_all_part2<X> ()
+  // x in s1 + s2 && x !in s1 ==> x in s2
+  ensures forall x: X, s1: AbSeq<X>, s2: AbSeq<X> :: AbSeqIn(x, AbSeqConcat(s1, s2)) && !AbSeqIn(x, s1) ==> AbSeqIn(x, s2)
+  { forall x, s1, s2 | AbSeqIn(x, AbSeqConcat(s1, s2)) && !AbSeqIn(x, s1)
+    { Seq_Props_concat_in_all_part2_p3<X>(x, s1, s2); } }
+
+lemma Seq_Props_concat_index_part1<X> ()
+  ensures forall i: AbInt, s1: AbSeq<X>, s2: AbSeq<X> ::
+  AbLeqLt(i, I0, AbSeqLen(s1)) ==> // 0 <= i < |s1|
+  AbLt(i, AbSeqLen(AbSeqConcat(s1, s2))) ==> // i < |s1| < |s1 + s2|
+  AbSeqIndex(i, s1) == AbSeqIndex(i, AbSeqConcat(s1, s2))
+  { forall i, s1, s2 | AbLeqLt(i, I0, AbSeqLen(s1)) && 
+      AbLt(i, AbSeqLen(AbSeqConcat(s1, s2)))
+    { Seq_Props_concat_index_part1_p3<X>(i, s1, s2); } }
+
+lemma Seq_Props_concat_index_part2<X> ()
+  ensures forall i: AbInt, s1: AbSeq<X>, s2: AbSeq<X> ::
+    AbLeqLt(i, I0, AbSeqLen(s2)) ==>
+    AbLeq(I0, AbAdd(i, AbSeqLen(s1))) ==> // 0 <= i + |s1|
+    AbLt(AbAdd(i, AbSeqLen(s1)), AbSeqLen(AbSeqConcat(s1, s2))) ==> // i + |s1| < |s1 + s2|
+    AbSeqIndex(i, s2) == AbSeqIndex(AbAdd(i, AbSeqLen(s1)), AbSeqConcat(s1, s2))
+  { forall i, s1, s2 | AbLeqLt(i, I0, AbSeqLen(s2)) && 
+      AbLeq(I0, AbAdd(i, AbSeqLen(s1))) && 
+      AbLt(AbAdd(i, AbSeqLen(s1)), AbSeqLen(AbSeqConcat(s1, s2)))
+    { Seq_Props_concat_index_part2_p3<X>(i, s1, s2); } }
+
+lemma Seq_Props_concat_is_orig<X> ()
+  ensures forall i: AbInt, s: AbSeq<X> ::
+    AbLeqLt(i, I0, AbSeqLen(s)) ==> // 0 <= i < |s|
+    s == AbSeqConcat(AbSeqSlice(I0, i, s), AbSeqSlice(i, AbSeqLen(s), s))
+  { forall i, s | AbLeqLt(i, I0, AbSeqLen(s))
+    { Seq_Props_concat_is_orig_p2<X> (i, s); } }
+
+lemma Seq_Props_in_empty<X> () // empty seq
+  ensures forall v: X, s: AbSeq<X> :: AbSeqLen(s) == I0 ==> !AbSeqIn(v, s)
+  {forall v, s | AbSeqLen(s) == I0
+    { Seq_Props_in_empty_p2<X>(v, s); } }
+
+lemma Seq_Props_in_non_empty<X> () // i in s ==> |s| > 0
+  ensures forall v: X, s: AbSeq<X> :: AbSeqIn(v, s) ==> AbLt(I0, AbSeqLen(s))
+  {forall v, s | AbSeqIn(v, s)
+    { Seq_Props_in_non_empty_p2<X>(v, s); } }
+
+lemma Seq_Props_in_idx<X> () // v in s ==> s[i] == v
+  ensures forall v: X, s: AbSeq<X> :: AbSeqIn(v, s) ==>
+    (exists i: AbInt :: AbLeqLt(i, I0, AbSeqLen(s)) && AbSeqIndex(i, s) == v )
+  { forall v, s | AbSeqIn(v, s)
+    { Seq_Props_in_idx_p2<X>(v, s); } }
+
+lemma Seq_Props_slice_in<X> ()
+  ensures forall i: AbInt, j: AbInt, s: AbSeq<X>, v: X ::
+    AbLeq(I0, i) && AbLeq(j, AbSeqLen(s)) && AbLeq(i, j) ==>
+    AbSeqIn(v, AbSeqSlice(i, j, s)) ==> AbSeqIn(v, s)
+  { forall i, j, s, v | AbLeq(I0, i) && AbLeq(j, AbSeqLen(s)) && AbLeq(i, j)
+    { Seq_Props_slice_in_p4<X>(i, j, s, v); } }
+
+lemma Seq_Props_index_props ()
+  ensures forall i: AbInt, j: AbInt, x: AbInt, s: AbSeq<AbInt>, s': AbSeq<AbInt> ::
+    ((AbLt(I0, i) || I0 == i) && AbLt(i, AbSeqLen(s)) && AbLt(AbSeqIndex(i, s), x)) ==> 
+    ((AbLt(I0, j) || I0 == j) && AbLt(j, AbSeqLen(s'))) ==>
+    (forall v :: AbSeqIn(v, s') ==> AbSeqIn(v, s)) ==>
+    AbLt(AbSeqIndex(j, s'), x)
+  ensures forall i: AbInt, j: AbInt, x: AbInt, s: AbSeq<AbInt>, s': AbSeq<AbInt> ::
+    ((AbLt(I0, i) || I0 == i) && AbLt(i, AbSeqLen(s)) && AbLt(x, AbSeqIndex(i, s))) ==> 
+    ((AbLt(I0, j) || I0 == j) && AbLt(j, AbSeqLen(s'))) ==>
+    (forall v :: AbSeqIn(v, s') ==> AbSeqIn(v, s)) ==>
+    AbLt(x, AbSeqIndex(j, s'))
+  // { }
